changes to the Plain files

examples/crypto/HyE.PlainAE.fst
@@ -12,9 +12,9 @@ open Platform.Bytes
    If it is an honest message, it encapsulates a (protected) hpke payload.
    If it is not an honest message, it is plain bytes.
 *)
-noeq abstract type protected_ae_plain (i:ae_id) = (
-  if pke_honest (fst i) && not ae_honest i && hpke_ind_cca then
-    p:protected_hpke_plain (fst i)
+abstract type protected_ae_plain (i:ae_id) = (
+  if pke_honest (fst i) && not (ae_honest i) && hpke_ind_cca then
+    protected_hpke_plain (fst i)
   else 
     hpke_plain
   )
@@ -23,10 +23,10 @@ type ae_plain = Bytes.bytes
 
 val length: #i:ae_id -> (protected_ae_plain i) -> Tot nat
 let length #i p = 
-  if ae_honest i && hpke_ind_cca then
-    PlainHPKE.length p.p
+  if pke_honest (fst i) && not (ae_honest i) && hpke_ind_cca then
+    PlainHPKE.length p
   else
-    length p.p
+    Bytes.length p
 
 (**
    Coerced messages can only be flagged as not honest.
@@ -39,35 +39,35 @@ let coerce #i p =
    We allow a transition from protected_ae_plain to ae_plain only if either there is no
    idealization or if if the message is not honest.
 *)
-val repr: #i:ae_id -> p:protected_ae_plain i{not ae_ind_cca || not (ae_honest i)} -> Tot (ae_plain_content i)
+val repr: #i:ae_id -> p:protected_ae_plain i{not ae_ind_cca || not (ae_honest i)} -> Tot (ae_plain)
 let repr #i p = 
   if ae_honest i && ae_ind_cca then
     PlainHPKE.repr p.p 
   else
     p.p
-
-(**
-   This is a helper function used by HPKE.encrypt to encapsulate the payload before
-   passing it on to AE.encrypt. If AE is idealized and the payload is honest, then we 
-   wrap the payload into our abstract type in good faith. If not, we coerce it.
-*)
-val ae_message_wrap: #i:ae_id -> p:ae_plain_content i -> Tot (protected_ae_plain i)
-let ae_message_wrap #i p =
-  if ae_honest i && ae_ind_cca then
-    Protected_ae_plain p
-  else
-    coerce p
-
-(**
-   This is the reverse function to ae_message_wrap. HPKE.decrypt uses it to extract a
-   protected ae payload. If it AE is idealized and the payload is honest, then
-   we strip it of its protection in good faith. Otherwise we break it down to its 
-   byte representation using repr.
-*)
-val ae_message_unwrap: #i:ae_id -> p:protected_ae_plain i -> Tot (ae_plain_content i)
-let ae_message_unwrap #i p =
-  if ae_honest i && ae_ind_cca then
-    p.p
-  else 
-repr p
+//
+//(**
+//   This is a helper function used by HPKE.encrypt to encapsulate the payload before
+//   passing it on to AE.encrypt. If AE is idealized and the payload is honest, then we 
+//   wrap the payload into our abstract type in good faith. If not, we coerce it.
+//*)
+//val ae_message_wrap: #i:ae_id -> p:protected_ae_plain i -> Tot (protected_ae_plain i)
+//let ae_message_wrap #i p =
+//  if ae_honest i && ae_ind_cca then
+//    Protected_ae_plain p
+//  else
+//    coerce p
+//
+//(**
+//   This is the reverse function to ae_message_wrap. HPKE.decrypt uses it to extract a
+//   protected ae payload. If it AE is idealized and the payload is honest, then
+//   we strip it of its protection in good faith. Otherwise we break it down to its 
+//   byte representation using repr.
+//*)
+//val ae_message_unwrap: #i:ae_id -> p:protected_ae_plain i -> Tot (ae_plain_content i)
+//let ae_message_unwrap #i p =
+//  if ae_honest i && ae_ind_cca then
+//    p.p
+//  else 
+//repr p
 
