examples/crypto/HyE.PlainHPKE.fst
@@ -13,17 +13,16 @@ open HyE.Indexing
 
 type hpke_plain = Bytes.bytes
 
-abstract type protected_hpke_plain (i:pke_id)= 
-  | Prot_hpke_p: b:hpke_plain -> protected_hpke_plain i
+abstract type protected_hpke_plain (i:pke_id) = hpke_plain
 
 (* two pure functions, never called when ideal *)
 val repr: #i:pke_id -> p:protected_hpke_plain i{not (pke_honest i) || not hpke_ind_cca} -> Tot (hpke_plain)
-let repr #i p = p.b
+let repr #i p = p
 
 // Change this if we want to use signcryption with hpke_int-ctxt
 val coerce: #i:pke_id -> p:hpke_plain{not (pke_honest i) || not hpke_ind_cca} -> Tot (protected_hpke_plain i)
 let coerce #i p = 
-  Prot_hpke_p #i p
+  p
 
 val length: #i:pke_id -> protected_hpke_plain i -> Tot nat
-let length #i p = Bytes.length p.b
+let length #i p = Bytes.length p
